ImplFlush verifies. Yay

disk-betree/ImplFlush.i.dfy
@@ -1,8 +1,9 @@
 include "ImplCache.i.dfy"
+include "ImplModelFlush.i.dfy"
 
 module ImplFlush { 
   import opened Impl
-  //import opened ImplCache
+  import opened ImplCache
 
   import opened Options
   import opened MainDiskIOHandler
@@ -13,123 +14,77 @@ module ImplFlush {
   import opened BucketsLib
 
   import opened NativeTypes
+  import ImplModel
+  import ImplModelCache
+  import ImplModelFlush
 
-  method flush(k: ImplConstants, s: ImplVariables, io: DiskIOHandler, ref: BT.G.Reference, slot: int)
+  method flush(k: ImplConstants, s: ImplVariables, io: DiskIOHandler, parentref: BT.G.Reference, slot: int)
   returns (s': ImplVariables)
+  requires IS.Inv(k, s)
   requires IS.WFVars(s)
   requires s.Ready?
-  requires ref in IS.IIndirectionTable(s.ephemeralIndirectionTable).graph
-  requires ref in s.cache
-  requires s.cache[ref].children.Some?
-  requires 0 <= slot < |s.cache[ref].buckets|
+  requires parentref in IS.IIndirectionTable(s.ephemeralIndirectionTable)
+  requires parentref in s.cache
+  requires s.cache[parentref].children.Some?
+  requires 0 <= slot < |s.cache[parentref].buckets|
   requires io.initialized()
   requires s.rootBucket == TTT.EmptyTree // FIXME we don't actually need this unless we're flushing the root
   modifies io
-  requires BBC.Inv(k, IS.IVars(s))
-  ensures IS.WFVars(s')
-  ensures ImplADM.M.Next(Ik(k), old(IS.IVars(s)), IS.IVars(s'), UI.NoOp, io.diskOp())
+  ensures IS.WVars(s')
+  ensures ImplModelFlush.flush(IS.Ic(k), old(IS.IVars(s)), old(IS.IIO(io)), parentref, slot) == (IS.IVars(s'), IS.IIO(io))
   // NOALIAS statically enforced no-aliasing would probably help here
   ensures forall r | r in s.ephemeralIndirectionTable.Repr :: fresh(r) || r in old(s.ephemeralIndirectionTable.Repr)
   modifies s.ephemeralIndirectionTable.Repr
   {
     if s.frozenIndirectionTable.Some? {
-      var lbaGraph := s.frozenIndirectionTable.value.Get(ref);
+      var lbaGraph := s.frozenIndirectionTable.value.Get(parentref);
       if lbaGraph.Some? {
-        assert ref in IS.IIndirectionTable(s.frozenIndirectionTable.value).graph;
         var (lba, _) := lbaGraph.value;
         if lba.None? {
-          assert ref !in IS.IIndirectionTable(s.frozenIndirectionTable.value).locs;
           s' := s;
-          assert noop(k, old(IS.IVars(s)), IS.IVars(s'));
           print "giving up; flush can't run because frozen isn't written";
           return;
         }
       }
     }
 
-    var node := s.cache[ref];
-
-    INodeRootEqINodeForEmptyRootBucket(node);
-
-    assert IS.INode(node) == IS.ICache(s.cache, s.rootBucket)[ref];
-    assert BT.WFNode(IS.INode(node));
-
+    var node := s.cache[parentref];
     var childref := node.children.value[slot];
-
-    assert childref in BT.G.Successors(IS.INode(node));
-
     if (childref !in s.cache) {
-      s' := PageInReq(k, s, io, childref);
+      ImplModelCache.lemmaChildInGraph(IS.Ic(k), IS.IVars(s), parentref, childref);
+      // trigger something in Inv about every child pointer points to allocated
+      // indirection record.
+      assert childref in ImplModel.IIndirectionTable(IS.IIndirectionTable(s.ephemeralIndirectionTable)).graph;
+      s' := ImplIO.PageInReq(k, s, io, childref);
       return;
     }
 
     var child := s.cache[childref];
-
-    INodeRootEqINodeForEmptyRootBucket(child);
-
-    assert IS.INode(child) == IS.ICache(s.cache, s.rootBucket)[childref];
-    assert BT.WFNode(IS.INode(child));
-
     if (!(
       && |node.buckets[slot].keys| < 0x4000_0000_0000_0000
       && |child.buckets| < 0x1_0000_0000_0000_0000
       && (forall i | 0 <= i < |child.buckets| :: |child.buckets[i].keys| < 0x4000_0000_0000_0000)
     )) {
       s' := s;
-      assert noop(k, old(IS.IVars(s)), IS.IVars(s'));
       print "giving up; data is 2 big\n";
       return;
     }
 
-    forall i, key | 0 <= i < |child.buckets| && key in KMTable.I(child.buckets[i]) ensures Pivots.Route(child.pivotTable, key) == i
-    {
-      //assert BT.NodeHasWFBucketAt(IS.INode(child), i);
-    }
-
     var newbuckets := KMTable.Flush(node.buckets[slot], child.buckets, child.pivotTable);
     var newchild := child.(buckets := newbuckets);
-
-    WFBucketListFlush(KMTable.I(node.buckets[slot]), KMTable.ISeq(child.buckets), child.pivotTable);
-
-    assert BT.G.Successors(IS.INode(newchild)) == BT.G.Successors(IS.INode(child));
-    assert BC.BlockPointsToValidReferences(IS.INode(newchild), IS.IIndirectionTable(s.ephemeralIndirectionTable).graph);
-
     var s1, newchildref := alloc(k, s, newchild);
     if newchildref.None? {
-      s' := s;
-      assert noop(k, old(IS.IVars(s)), IS.IVars(s'));
-      print "giving up; could not get ref\n";
+      s' := s1;
+      print "giving up; could not get parentref\n";
       return;
     }
-    ghost var s1Interpreted := IS.IVars(s1);
 
-    var newparent := IS.Node(
+    var newparent := IS.IM.Node(
         node.pivotTable,
         Some(node.children.value[slot := newchildref.value]),
         node.buckets[slot := KMTable.Empty()]
       );
 
-    assert BC.BlockPointsToValidReferences(IS.INode(node), IS.IIndirectionTable(s1.ephemeralIndirectionTable).graph);
-    forall ref | ref in BT.G.Successors(IS.INode(newparent)) ensures ref in IS.IIndirectionTable(s1.ephemeralIndirectionTable).graph {
-      if (ref == newchildref.value) {
-      } else {
-        assert ref in BT.G.Successors(IS.INode(node));
-      }
-    }
-    assert BC.BlockPointsToValidReferences(IS.INode(newparent), IS.IIndirectionTable(s1.ephemeralIndirectionTable).graph);
-
-    assert ref in s.cache;
-    assert ref in IS.ICache(s.cache, s.rootBucket);
-    assert ref in IS.ICache(s1.cache, s1.rootBucket);
-    assert ref in s1.cache;
-
-    s' := write(k, s1, ref, newparent);
-
-    ghost var flushStep := BT.NodeFlush(ref, IS.INode(node), childref, IS.INode(child), newchildref.value, IS.INode(newchild), slot);
-    assert BT.ValidFlush(flushStep);
-    ghost var step := BT.BetreeFlush(flushStep);
-    assert IS.INode(newparent) == BT.FlushOps(flushStep)[1].node;
-    BC.MakeTransaction2(k, old(IS.IVars(s)), s1Interpreted, IS.IVars(s'), BT.BetreeStepOps(step));
-    assert stepsBetree(k, old(IS.IVars(s)), IS.IVars(s'), UI.NoOp, step);
+    s' := write(k, s1, parentref, newparent);
   }
 }
